Coinduction.lean
@@ -1,0 +1,100 @@
+import Lean
+
+namespace Coinduction
+
+set_option autoImplicit false
+
+/-
+codata Stream (α : Type u) : Type u where
+  hd : α
+  tl : Stream α
+-/
+
+inductive Stream.Approx.{u} (α : Type u) : (ℓ : Nat) → Type u
+  | «⋯» : Approx α .zero
+  | mk {ℓ} (hd : α) (tl : Approx α ℓ) : Approx α ℓ.succ
+
+inductive Stream.Approx.Agree.{u} {α : Type u} : ∀ {ℓ₁ ℓ₂}, (x₁ : Approx α ℓ₁) → (x₂ : Approx α ℓ₂) → Prop
+  | «⋯» {ℓ₂} {x₂ : Approx α ℓ₂} : Agree .«⋯» x₂
+  | mk {ℓ₁ ℓ₂} {hd : α} {tl₁ : Approx α ℓ₁} {tl₂ : Approx α ℓ₂} (tl : Agree tl₁ tl₂) : Agree (.mk hd tl₁) (.mk hd tl₂)
+
+def Stream.{u} (α : Type u) : Type u :=
+  { f : (ℓ : Nat) → Stream.Approx α ℓ // ∀ ℓ, (f ℓ).Agree (f ℓ.succ) }
+
+def Stream.hd.{u} {α : Type u} (self : Stream α) : α :=
+  let .mk hd _ := self.val (.succ .zero); hd
+
+def Stream.tl.{u} {α : Type u} (self : Stream α) : Stream α where
+  val ℓ := let .mk _ tl := self.val ℓ.succ; tl
+  property ℓ := by
+    have := self.property ℓ.succ
+    dsimp only
+    generalize self.val ℓ.succ = x₁ at this
+    generalize self.val ℓ.succ.succ = x₂ at this
+    cases x₁ with | mk tl₁ =>
+    cases x₂ with | mk tl₂ =>
+    cases this with | mk tl =>
+    exact tl
+
+def Stream.corec.{s, u} {σ : Sort s} {α : Type u} (hd : (s : σ) → α) (tl : (s : σ) → σ) (s : σ) : Stream α where
+  val ℓ := @Nat.rec (fun ℓ => (s : σ) → Approx α ℓ) (fun _ => .«⋯») (fun _ f s => .mk (hd s) (f (tl s))) ℓ s
+  property ℓ := Nat.rec (fun _ => .«⋯») (fun _ h s => .mk (h (tl s))) ℓ s
+
+theorem Stream.hd_corec.{s, u} {σ : Sort s} {α : Type u} (hd : (s : σ) → α) (tl : (s : σ) → σ) (s : σ) : Stream.hd (corec hd tl s) = hd s := rfl
+theorem Stream.tl_corec.{s, u} {σ : Sort s} {α : Type u} (hd : (s : σ) → α) (tl : (s : σ) → σ) (s : σ) : Stream.tl (corec hd tl s) = corec hd tl (tl s) := rfl
+
+def rep.{u} {α : Type u} (x : α) : Stream α :=
+  .corec (fun _ => x) (·) ()
+
+def even.{u} {α : Type u} (xs : Stream α) : Stream α :=
+  .corec (fun xs => xs.hd) (fun xs => xs.tl.tl) xs
+
+def odd.{u} {α : Type u} (xs : Stream α) : Stream α :=
+  even xs.tl
+
+def merge.{u} {α : Type u} (xs ys : Stream α) : Stream α :=
+  .corec (fun (xs, _) => xs.hd) (fun (xs, ys) => (ys, xs.tl)) (xs, ys)
+
+/-
+codata Stream.Eq.{u} {α : Type u} (xs ys : Stream α) : Type u where
+  hd : xs.hd = ys.hd
+  tl : Eq xs.tl ys.tl
+-/
+
+inductive Stream.Eq.Approx.{u} {α : Type u} : (xs ys : Stream α) → (ℓ : Nat) → Prop where
+  | «⋯» {xs ys} : Approx xs ys .zero
+  | mk {ℓ xs ys} (hd : xs.hd = ys.hd) (tl : Approx xs.tl ys.tl ℓ) : Approx xs ys ℓ.succ
+
+/-
+inductive Stream.Eq.Approx.Agree.{u} {α : Type u} : {xs ys : Stream α} → ∀ {ℓ₁ ℓ₂}, (x₁ : Approx xs ys ℓ₁) → (x₂ : Approx xs ys ℓ₂) → Prop
+  | «⋯» {ℓ₂ xs ys} (x₂ : Approx xs ys ℓ₂) : Agree .«⋯» x₂
+  | mk {ℓ₁ ℓ₂} {xs ys : Stream α} {hd : xs.hd = ys.hd} {tl₁ : Approx xs.tl ys.tl ℓ₁} {tl₂ : Approx xs.tl ys.tl ℓ₂} (tl : Agree tl₁ tl₂) : Agree (.mk hd tl₁) (.mk hd tl₂)
+-/
+
+def Stream.Eq.{u} {α : Type u} (xs ys : Stream α) : Prop :=
+  (ℓ : Nat) → Eq.Approx xs ys ℓ
+
+def Stream.Eq.hd.{u} {α : Type u} {xs ys : Stream α} (self : Eq xs ys) : xs.hd = ys.hd :=
+  let .mk hd _ := self (.succ .zero); hd
+
+def Stream.Eq.tl.{u} {α : Type u} {xs ys : Stream α} (self : Eq xs ys) : Eq xs.tl ys.tl
+  | ℓ => let .mk _ tl := self ℓ.succ; tl
+
+def Stream.Eq.corec.{s, u} {α : Type u} {σ : (xs ys : Stream α) → Sort s} (hd : ∀ {xs ys}, (s : σ xs ys) → xs.hd = ys.hd) (tl : ∀ {xs ys}, (s : σ xs ys) → σ xs.tl ys.tl) {xs ys : Stream α} (s : σ xs ys) : Eq xs ys
+  | ℓ => @Nat.rec (fun ℓ => ∀ {xs ys}, (s : σ xs ys) → Approx xs ys ℓ) (fun _ => .«⋯») (fun _ f _ _ s => .mk (hd s) (f (tl s))) ℓ xs ys s
+
+theorem merge_even_odd.{u} {α : Type u} (xs : Stream α) : Stream.Eq xs (merge (even xs) (odd xs)) :=
+  .corec (σ := fun xs ys => merge (even xs) (odd xs) = ys) (fun | .refl _ => rfl) (fun | .refl _ => rfl) rfl
+
+/-
+mutual
+
+inductive SP.{u, v} (α : Type u) (β : Type v) : Type (max u v)
+  | get (f : α → SP α β)
+  | put (b : β) (sp : SP' α β)
+
+codata SP'.{u, v} (α : Type u) (β : Type v) : Type (max u v) where
+  force : SP α β
+
+end
+-/
