rec/lakefile.lean
@@ -1,7 +1,0 @@
-import Lake
-open Lake DSL
-
-package rec
-
-@[default_target]
-lean_lib Rec
